Add type check to is derivable back

theories/glogic.v
@@ -39,8 +39,179 @@ Module GLogic (SqSet : SQ_SET).
   }.
   *)
 
-  Definition wf_sequent C (p : sq_set) j :=
-    has_type C j ty_prp /\ forall t, t ∈ p -> has_type C t ty_prp.
+  Definition is_form C t := has_type C t ty_prp.
+  Definition wf_sq_set C (l : sq_set) := forall t, t ∈ l -> has_type C t ty_prp.
+
+  Definition wf_sequent C (p : sq_set) c := wf_sq_set C p /\ is_form C c.
+
+  Inductive is_derivable_wf : context -> sq_set -> tm -> Prop :=
+    | wrl_set C l m c :
+        l ≡ m ->
+        is_derivable_wf C l c ->
+        is_derivable_wf C m c
+    | wrl_id C a b :
+        has_type C a ty_prp ->
+        has_type C b ty_prp ->
+        tm_equiv C a b ->
+        is_derivable_wf C {[a]} b
+    | wrl_cut C l m b c :
+        is_derivable_wf C l b ->
+        is_derivable_wf C (m ∪ {[b]}) c ->
+        is_derivable_wf C (l ∪ m) c
+    | wrl_cL C l b c :
+        is_derivable_wf C (l ∪ {[b; b]}) c ->
+        is_derivable_wf C (l ∪ {[b]}) c
+    | wrl_wL C l m b :
+        (forall a, a ∈ l -> has_type C a ty_prp) ->
+        is_derivable_wf C m b ->
+        is_derivable_wf C (l ∪ m) b
+    | wrl_botL C c :
+        has_type C c ty_prp ->
+        is_derivable_wf C {[gtm_bot]} c
+    | wrl_topR C :
+        is_derivable_wf C ∅ gtm_top
+    | wrl_orL C l b c d :
+        is_derivable_wf C (l ∪ {[b]}) c ->
+        is_derivable_wf C (l ∪ {[d]}) c ->
+        is_derivable_wf C (l ∪ {[ <{ b \/ d }> ]}) c
+    | wrl_orR1 C l b c :
+        has_type C c ty_prp ->
+        is_derivable_wf C l b ->
+        is_derivable_wf C l <{ b \/ c }>
+    | wrl_orR2 C l b c :
+        has_type C b ty_prp ->
+        is_derivable_wf C l c ->
+        is_derivable_wf C l <{ b \/ c }>
+    | wrl_andL1 C l b c d :
+        has_type C d ty_prp ->
+        is_derivable_wf C (l ∪ {[b]}) c ->
+        is_derivable_wf C (l ∪ {[ <{ b /\ d }> ]}) c
+    | wrl_andL2 C l b c d :
+        has_type C b ty_prp ->
+        is_derivable_wf C (l ∪ {[d]}) c ->
+        is_derivable_wf C (l ∪ {[ <{ b /\ d }> ]}) c
+    | wrl_andR C l b c :
+        is_derivable_wf C l b ->
+        is_derivable_wf C l c ->
+        is_derivable_wf C l <{ b /\ c }>
+    | wrl_impL C l b c d :
+        is_derivable_wf C l b ->
+        is_derivable_wf C (l ∪ {[d]}) c ->
+        is_derivable_wf C (l ∪ {[ <{ b > d }> ]}) c
+    | wrl_impR C l b c :
+        is_derivable_wf C (l ∪ {[b]}) c ->
+        is_derivable_wf C l <{ b > c }>
+    | wrl_forL C T l b c t :
+        has_type C t T ->
+        is_derivable_wf C (l ∪ {[ subst_last C C t b ]}) c ->
+        is_derivable_wf C (l ∪ {[ <{for T, b}> ]}) c
+    | wrl_forR C T l b sb :
+        (forall t, t ∈ sb <-> in_supp b t) ->
+        is_derivable_wf (C +: foldr ty_arr T (type_check_other <$> sb)) (sq_set_map (lift C) l) (
+          subst_last C (S C) (foldl tm_app (tm_lvl C) sb) b
+        ) ->
+        is_derivable_wf C l <{for T, b}>
+    | wrl_exL C T l b c sb :
+        (forall t, t ∈ sb <-> in_supp b t) ->
+        is_derivable_wf (C +: foldr ty_arr T (type_check_other <$> sb)) (
+          sq_set_map (lift C) l ∪
+          {[subst_last C (S C) (foldl tm_app (tm_lvl C) sb) b]}
+        ) (lift C c) ->
+        is_derivable_wf C (l ∪ {[ <{ex T, b}> ]}) c
+    | wrl_exR C T l b t :
+        has_type C t T ->
+        is_derivable_wf C l (subst_last C C t b) ->
+        is_derivable_wf C l <{ex T, b}>
+    | wrl_nabL {T b} n (_ : ~ in_supp b (gtm_nom T n)) C l c :
+        is_derivable_wf C (l ∪ {[ subst_last C C (gtm_nom T n) b ]}) c ->
+        is_derivable_wf C (l ∪ {[ <{nab T, b}> ]}) c
+    | wrl_nabR {T b} n (_ : ~ in_supp b (gtm_nom T n)) C l :
+        is_derivable_wf C l (subst_last C C (gtm_nom T n) b) ->
+        is_derivable_wf C l (<{nab T, b}>)
+  .
+
+  Theorem has_type_fold C T h l t :
+    Forall2 (fun x X => has_type C x X) l h ->
+    has_type C t (foldr ty_arr T h) ->
+    has_type C (foldl tm_app t l) T.
+  Proof.
+    revert h t. induction l; intros h t F Ht.
+    - inversion F. now subst.
+    - simpl. destruct h; inversion F. subst.
+      eapply IHl; try eassumption.
+      tm_simpl. now exists t0.
+  Qed.
+
+  Theorem has_type_fold2 C T sb b :
+    (forall t, t ∈ sb -> in_supp b t) ->
+    has_type (C +: foldr ty_arr T (type_check_other <$> sb)) (subst_last C (S C) (foldl tm_app (tm_lvl C) sb) b) -[ o ]- ->
+    has_type (C +: T) b ty_prp.
+  Proof.
+    intros.
+    eapply (has_type_subst_last2 _ (C +: foldr ty_arr T (type_check_other <$> sb)));
+      simpl; try eassumption; try lia.
+    - intros. now rewrite decide_True.
+    - eapply has_type_fold; tm_simpl; [|rewrite decide_False; intuition lia].
+      remember (C +: foldr ty_arr T (type_check_other <$> sb)) as D eqn : ED.
+      clear ED H0. induction sb; simpl in *; constructor.
+      + constructor. set_unfold. eapply in_supp_other. auto.
+      + set_unfold. auto.
+  Qed.
+  Theorem is_derivable_wf_wf C l c : is_derivable_wf C l c -> wf_sequent C l c.
+  Proof.
+    intros D. unfold wf_sequent. induction D; simpl in *.
+    - set_unfold. intuition. apply H0. now apply H.
+    - split; try assumption.
+      intros. set_unfold. congruence.
+    - set_unfold. intuition.
+    - set_unfold. intuition.
+    - set_unfold. intuition.
+    - set_unfold. intuition. subst. now constructor.
+    - set_unfold. intuition. now constructor.
+    - set_unfold. intuition. subst.
+      repeat eapply ht_app; auto. now apply ht_other2.
+    - intuition. repeat eapply ht_app; try eassumption. now apply ht_other2.
+    - intuition. repeat eapply ht_app; try eassumption. now apply ht_other2.
+    - set_unfold. intuition. subst.
+      repeat eapply ht_app; eauto. now apply ht_other2.
+    - set_unfold. intuition. subst.
+      repeat eapply ht_app; eauto. now apply ht_other2.
+    - intuition. repeat eapply ht_app; try eassumption. now apply ht_other2.
+    - set_unfold. intuition. subst.
+      repeat eapply ht_app; eauto. now apply ht_other2.
+    - set_unfold. intuition.
+      repeat eapply ht_app; eauto. now apply ht_other2.
+    - set_unfold. intuition. subst. econstructor.
+      + now apply ht_other2.
+      + tm_simpl. eexists; try reflexivity.
+        eapply has_type_subst_last2; eauto.
+    - unfold wf_sq_set. intuition; [|econstructor].
+      + eapply has_type_lift2.
+        apply H0. apply sq_set_map_spec. eauto.
+      + now apply ht_other2.
+      + tm_simpl. eexists; intuition.
+        eapply has_type_fold2; try eassumption. apply H.
+    - set_unfold. intuition.
+      + eapply has_type_lift2. apply H0. left.
+        apply sq_set_map_spec. eauto.
+      + subst. econstructor; [now apply ht_other2|].
+        tm_simpl. eexists; try reflexivity.
+        eapply has_type_fold2; auto. apply H.
+      + eapply has_type_lift2; eassumption.
+    - intuition. econstructor; [now apply ht_other2|].
+      tm_simpl. eexists; [|reflexivity].
+      eapply has_type_subst_last2; eauto.
+    - set_unfold. intuition. subst.
+      econstructor; [now apply ht_other2|].
+      tm_simpl. eexists; [|reflexivity].
+      eapply has_type_subst_last2; eauto.
+      now constructor.
+    - intuition. econstructor; [now apply ht_other2|].
+      tm_simpl. eexists; [|reflexivity].
+      eapply has_type_subst_last2; eauto.
+      now constructor.
+  Qed.
+
 
   Inductive is_derivable : context -> sq_set -> tm -> Prop :=
     | rl_set C l m c :
@@ -121,99 +292,40 @@ Module GLogic (SqSet : SQ_SET).
   Notation "[{ sig ; l --> B }]" := (is_derivable sig l B)
     (sig custom stlc_ty, l custom stlc_tm, B custom stlc_tm) : stlc_scope.
 
-
-  (*
-  Theorem has_type_fold C T h l t :
-    Forall2 (fun x X => has_type C x X) l h ->
-    has_type C t (foldr ty_arr T h) ->
-    has_type C (foldl tm_app t l) T.
-  Proof.
-    revert h t. induction l; intros h t F Ht.
-    - inversion F. now subst.
-    - simpl. destruct h; inversion F. subst.
-      eapply IHl; try eassumption.
-      tm_simpl. now exists t0.
-  Qed.
-
-  Theorem has_type_fold2 C T sb b :
-    (forall t, t ∈ sb -> in_supp b t) ->
-    has_type (C +: foldr ty_arr T (type_check_other <$> sb)) (subst_last C (S C) (foldl tm_app (tm_lvl C) sb) b) -[ o ]- ->
-    has_type (C +: T) b ty_prp.
-  Proof.
-    intros.
-    eapply (has_type_subst_last2 _ (C +: foldr ty_arr T (type_check_other <$> sb)));
-      simpl; try eassumption; try lia.
-    - intros. now rewrite decide_True.
-    - eapply has_type_fold; tm_simpl; [|rewrite decide_False; intuition lia].
-      remember (C +: foldr ty_arr T (type_check_other <$> sb)) as D eqn : ED.
-      clear ED H0. induction sb; simpl in *; constructor.
-      + constructor. set_unfold. eapply in_supp_other. auto.
-      + set_unfold. auto.
-  Qed.
-
-  Theorem is_derivable_wf C l c : is_derivable C l c -> wf_sequent C l c.
-  Proof.
-    intros D. unfold wf_sequent. induction D; simpl in *.
-    - set_unfold. intuition. apply H1. now apply H.
-    - split; try assumption.
-      intros. set_unfold. congruence.
-    - set_unfold. intuition.
-    - set_unfold. intuition.
-    - set_unfold. intuition.
-    - set_unfold. intuition. subst. now constructor.
-    - set_unfold. intuition. now constructor.
-    - set_unfold. intuition. subst.
-      repeat eapply ht_app; auto. now apply ht_other2.
-    - intuition. repeat eapply ht_app; try eassumption. now apply ht_other2.
-    - intuition. repeat eapply ht_app; try eassumption. now apply ht_other2.
-    - set_unfold. intuition. subst.
-      repeat eapply ht_app; eauto. now apply ht_other2.
-    - set_unfold. intuition. subst.
-      repeat eapply ht_app; eauto. now apply ht_other2.
-    - intuition. repeat eapply ht_app; try eassumption. now apply ht_other2.
-    - set_unfold. intuition. subst.
-      repeat eapply ht_app; eauto. now apply ht_other2.
-    - set_unfold. intuition.
-      repeat eapply ht_app; eauto. now apply ht_other2.
-    - set_unfold. intuition. subst. econstructor.
-      + now apply ht_other2.
-      + tm_simpl. eexists; try reflexivity.
-        eapply has_type_subst_last2; eauto.
-    - intuition; [econstructor|].
-      + now apply ht_other2.
-      + tm_simpl. eexists; intuition.
-        eapply has_type_fold2; try eassumption. apply H.
-      + eapply has_type_lift2.
-        apply H1. apply sq_set_map_spec. eauto.
-    - set_unfold. intuition.
-      + eapply has_type_lift2; eassumption.
-      + eapply has_type_lift2. apply H1. left.
-        apply sq_set_map_spec. eauto.
-      + subst. econstructor; [now apply ht_other2|].
-        tm_simpl. eexists; try reflexivity.
-        eapply has_type_fold2; auto. apply H.
-    - intuition. econstructor; [now apply ht_other2|].
-      tm_simpl. eexists; [|reflexivity].
-      eapply has_type_subst_last2; eauto.
-    - set_unfold. intuition. subst.
-      econstructor; [now apply ht_other2|].
-      tm_simpl. eexists; [|reflexivity].
-      eapply has_type_subst_last2; eauto.
-      now constructor.
-    - intuition. econstructor; [now apply ht_other2|].
-      tm_simpl. eexists; [|reflexivity].
-      eapply has_type_subst_last2; eauto.
-      now constructor.
-  Qed.
-  *)
-
-
-
   Notation "∅" := empty (in custom stlc_ty) : stlc_scope.
   Notation "∅" := empty (in custom stlc_tm) : stlc_scope.
   Notation "s +: x" := (s ∪ {[x]}) (in custom stlc_tm at level 50, left associativity) : stlc_scope.
   Notation "∅" := empty : stdpp_scope.
   Notation "{[ x ]}" := (singleton x) (in custom stlc_tm) : stlc_scope.
+
+  Theorem union_empty (X : sq_set) : ∅ ∪ X ≡ X.
+  Proof. set_unfold. intuition. Qed.
+
+  Instance is_derivable_Proper : Proper ((=) ==> (≡) ==> (=) ==> iff) is_derivable.
+  Proof.
+    intros ? ** ? ** ? **. subst.
+    split; intros H; eapply rl_set; try apply H; easy.
+  Qed.
+
+
+  Theorem is_derivable_wf_is_derivable C l c :
+    is_derivable_wf C l c -> [{ C; l --> c }].
+  Proof.
+    intros DW. induction DW; subst.
+    - eapply rl_set; eassumption.
+    - rewrite <- union_empty. now apply rl_id.
+    - eapply rl_cut; try eassumption.
+      apply is_derivable_wf_wf in DW1. destruct DW1. assumption.
+    - now apply rl_cL.
+  Abort.
+
+  Theorem is_derivable_is_derivable_wf C l c :
+    wf_sequent C l c ->  [{ C; l --> c }] -> is_derivable_wf C l c.
+  Proof.
+    intros W D. induction D.
+    - eapply wrl_set; [eassumption|].
+  Abort.
+
 
   Theorem nom_in_supp b T : exists a, ~ in_supp b (gtm_nom T a).
   Proof. eexists. apply nom_fresh_in_supp. Qed.
@@ -235,15 +347,6 @@ Module GLogic (SqSet : SQ_SET).
   Theorem sq_set_swap (l : sq_set) a b :
     <{ l +: a +: b }> ≡ <{ l +: b +: a }>.
   Proof. set_unfold. intuition. Qed.
-
-  Theorem union_empty (X : sq_set) : ∅ ∪ X ≡ X.
-  Proof. set_unfold. intuition. Qed.
-
-  Instance is_derivable_Proper : Proper ((=) ==> (≡) ==> (=) ==> iff) is_derivable.
-  Proof.
-    intros ? ** ? ** ? **. subst.
-    split; intros H; eapply rl_set; try apply H; easy.
-  Qed.
 
   Theorem contrapositive C l b c :
     [{ C ; l +: b --> c }] -> [{ C ; l +: ~ c --> ~ b }].
